thys/AWN/OAWN_SOS_Labels.thy
@@ -12,7 +12,7 @@ begin
 lemma oelimder_guard:
   assumes "p = {l}\<langle>fg\<rangle> qq"
       and "l' \<in> labels \<Gamma> q"
-      and "((\<sigma>, p), a, (\<sigma>', q)) \<in> oseqp_sos \<Gamma>\<^sub>A\<^sub>O\<^sub>D\<^sub>V i"
+      and "((\<sigma>, p), a, (\<sigma>', q)) \<in> oseqp_sos \<Gamma> i"
   obtains p' where "p = {l}\<langle>fg\<rangle> p'"
                and "l' \<in> labels \<Gamma> qq"
   using assms by auto
@@ -20,7 +20,7 @@ lemma oelimder_guard:
 lemma oelimder_assign:
   assumes "p = {l}\<lbrakk>fa\<rbrakk> qq"
       and "l' \<in> labels \<Gamma> q"
-      and "((\<sigma>, p), a, (\<sigma>', q)) \<in> oseqp_sos \<Gamma>\<^sub>A\<^sub>O\<^sub>D\<^sub>V i"
+      and "((\<sigma>, p), a, (\<sigma>', q)) \<in> oseqp_sos \<Gamma> i"
   obtains p' where "p = {l}\<lbrakk>fa\<rbrakk> p'"
                and "l' \<in> labels \<Gamma> qq"
   using assms by auto
@@ -28,7 +28,7 @@ lemma oelimder_assign:
 lemma oelimder_ucast:
   assumes "p = {l}unicast(fip, fmsg).q1 \<triangleright> q2"
       and "l' \<in> labels \<Gamma> q"
-      and "((\<sigma>, p), a, (\<sigma>', q)) \<in> oseqp_sos \<Gamma>\<^sub>A\<^sub>O\<^sub>D\<^sub>V i"
+      and "((\<sigma>, p), a, (\<sigma>', q)) \<in> oseqp_sos \<Gamma> i"
   obtains p' pp' where "p = {l}unicast(fip, fmsg).p' \<triangleright> pp'"
                    and "case a of unicast _ _ \<Rightarrow> l' \<in> labels \<Gamma> q1
                                         | _ \<Rightarrow> l' \<in> labels \<Gamma> q2"
@@ -37,7 +37,7 @@ lemma oelimder_ucast:
 lemma oelimder_bcast:
   assumes "p = {l}broadcast(fmsg).qq"
       and "l' \<in> labels \<Gamma> q"
-      and "((\<sigma>, p), a, (\<sigma>', q)) \<in> oseqp_sos \<Gamma>\<^sub>A\<^sub>O\<^sub>D\<^sub>V i"
+      and "((\<sigma>, p), a, (\<sigma>', q)) \<in> oseqp_sos \<Gamma> i"
   obtains p' where "p = {l}broadcast(fmsg). p'"
                and "l' \<in> labels \<Gamma> qq"
   using assms by auto
@@ -45,7 +45,7 @@ lemma oelimder_bcast:
 lemma oelimder_gcast:
   assumes "p = {l}groupcast(fips, fmsg).qq"
       and "l' \<in> labels \<Gamma> q"
-      and "((\<sigma>, p), a, (\<sigma>', q)) \<in> oseqp_sos \<Gamma>\<^sub>A\<^sub>O\<^sub>D\<^sub>V i"
+      and "((\<sigma>, p), a, (\<sigma>', q)) \<in> oseqp_sos \<Gamma> i"
   obtains p' where "p = {l}groupcast(fips, fmsg). p'"
                and "l' \<in> labels \<Gamma> qq"
   using assms by auto
@@ -53,7 +53,7 @@ lemma oelimder_gcast:
 lemma oelimder_send:
   assumes "p = {l}send(fmsg).qq"
       and "l' \<in> labels \<Gamma> q"
-      and "((\<sigma>, p), a, (\<sigma>', q)) \<in> oseqp_sos \<Gamma>\<^sub>A\<^sub>O\<^sub>D\<^sub>V i"
+      and "((\<sigma>, p), a, (\<sigma>', q)) \<in> oseqp_sos \<Gamma> i"
   obtains p' where "p = {l}send(fmsg). p'"
                and "l' \<in> labels \<Gamma> qq"
   using assms by auto
@@ -61,7 +61,7 @@ lemma oelimder_send:
 lemma oelimder_deliver:
   assumes "p = {l}deliver(fdata).qq"
       and "l' \<in> labels \<Gamma> q"
-      and "((\<sigma>, p), a, (\<sigma>', q)) \<in> oseqp_sos \<Gamma>\<^sub>A\<^sub>O\<^sub>D\<^sub>V i"
+      and "((\<sigma>, p), a, (\<sigma>', q)) \<in> oseqp_sos \<Gamma> i"
   obtains p' where "p = {l}deliver(fdata).p'"
                and "l' \<in> labels \<Gamma> qq"
   using assms by auto
@@ -69,7 +69,7 @@ lemma oelimder_deliver:
 lemma oelimder_receive:
   assumes "p = {l}receive(fmsg).qq"
       and "l' \<in> labels \<Gamma> q"
-      and "((\<sigma>, p), a, (\<sigma>', q)) \<in> oseqp_sos \<Gamma>\<^sub>A\<^sub>O\<^sub>D\<^sub>V i"
+      and "((\<sigma>, p), a, (\<sigma>', q)) \<in> oseqp_sos \<Gamma> i"
   obtains p' where "p = {l}receive(fmsg).p'"
                and "l' \<in> labels \<Gamma> qq"
   using assms by auto
